code/ecdsa/Hacl.Impl.EC.LowLevel.fst
@@ -436,14 +436,7 @@ val felem_double_p256: a: felem P256 -> out: felem P256 ->
       as_nat P256 h1 out == (2 * as_nat P256 h0 a) % getPrime P256 /\
       as_nat P256 h1 out == toDomain #P256 (2 * fromDomain #P256 (as_nat P256 h0 a) % getPrime P256)))
 
-let felem_double_p256 arg1 out =
-  let h0 = ST.get() in
-
-  let t = add_bn arg1 arg1 out in
-  reduction_prime_2prime_with_carry_cin t out out;
-
-  additionInDomain #P256 #DH (as_nat P256 h0 arg1) (as_nat P256 h0 arg1);
-  inDomain_mod_is_not_mod #P256 #DH (fromDomain #P256 (as_nat P256 h0 arg1) + fromDomain #P256 (as_nat P256 h0 arg1))
+let felem_double_p256 arg1 out = felem_double_ #P256 arg1 out
 
 
 val felem_double_p384: a: felem P384 -> out: felem P384 ->
@@ -455,14 +448,7 @@ val felem_double_p384: a: felem P384 -> out: felem P384 ->
       as_nat P384 h1 out == (2 * as_nat P384 h0 a) % getPrime P384 /\
       as_nat P384 h1 out == toDomain #P384 (2 * fromDomain #P384 (as_nat P384 h0 a) % getPrime P384)))
 
-let felem_double_p384 arg1 out =
-  let h0 = ST.get() in
-
-  let t = add_bn arg1 arg1 out in
-  reduction_prime_2prime_with_carry_cin t out out;
-
-  additionInDomain #P384 #DH (as_nat P384 h0 arg1) (as_nat P384 h0 arg1);
-  inDomain_mod_is_not_mod #P384 #DH (fromDomain #P384 (as_nat P384 h0 arg1) + fromDomain #P384 (as_nat P384 h0 arg1))
+let felem_double_p384 arg1 out = felem_double_ #P384 arg1 out
 
 
 val felem_double_generic: a: felem Default -> out: felem Default ->
@@ -474,14 +460,7 @@ val felem_double_generic: a: felem Default -> out: felem Default ->
       as_nat Default h1 out == (2 * as_nat Default h0 a) % getPrime Default /\
       as_nat Default h1 out == toDomain #Default (2 * fromDomain #Default (as_nat Default h0 a) % getPrime Default)))
 
-let felem_double_generic arg1 out =
-  let h0 = ST.get() in
-
-  let t = add_bn arg1 arg1 out in
-  reduction_prime_2prime_with_carry_cin t out out;
-
-  additionInDomain #Default #DH (as_nat Default h0 arg1) (as_nat Default h0 arg1);
-  inDomain_mod_is_not_mod #Default #DH (fromDomain #Default (as_nat Default h0 arg1) + fromDomain #Default (as_nat Default h0 arg1))
+let felem_double_generic arg1 out = felem_double_ #Default arg1 out
 
 
 let felem_double #c arg1 out = 
@@ -494,7 +473,17 @@ let felem_double #c arg1 out =
 #set-options "--fuel 1 --ifuel 1 --z3rlimit 200"
 
 
-let felem_sub #c arg1 arg2 out =
+inline_for_extraction noextract
+val felem_sub_: #c: curve -> a: felem c -> b: felem c -> out: felem c ->
+  Stack unit
+  (requires (fun h0 ->
+    live h0 out /\ live h0 a /\ live h0 b /\ eq_or_disjoint a out /\ eq_or_disjoint b out /\ eq_or_disjoint a b /\
+    as_nat c h0 a < getPrime c /\ as_nat c h0 b < getPrime c))
+  (ensures (fun h0 _ h1 -> modifies (loc out) h0 h1 /\
+    as_nat c h1 out == (as_nat c h0 a - as_nat c h0 b) % getPrime c /\
+    as_nat c h1 out == toDomain #c ((fromDomain #c (as_nat c h0 a) - fromDomain #c (as_nat c h0 b)) % getPrime c)))
+
+let felem_sub_ #c arg1 arg2 out =
     let h0 = ST.get() in
   let t = sub_bn arg1 arg2 out in
     let h1 = ST.get() in 
@@ -527,6 +516,50 @@ let felem_sub #c arg1 arg2 out =
 
   substractionInDomain #c #DH (as_nat c h0 arg1) (as_nat c h0 arg2); 
   inDomain_mod_is_not_mod #c #DH (fromDomain #c (as_nat c h0 arg1) - fromDomain #c (as_nat c h0 arg2))
+
+
+val felem_sub_p256: a: felem P256 -> b: felem P256 -> out: felem P256 ->
+  Stack unit
+  (requires (fun h0 ->
+    live h0 out /\ live h0 a /\ live h0 b /\ eq_or_disjoint a out /\ eq_or_disjoint b out /\ eq_or_disjoint a b /\
+    as_nat P256 h0 a < getPrime P256 /\ as_nat P256 h0 b < getPrime P256))
+  (ensures (fun h0 _ h1 -> modifies (loc out) h0 h1 /\
+    as_nat P256 h1 out == (as_nat P256 h0 a - as_nat P256 h0 b) % getPrime P256 /\
+    as_nat P256 h1 out == toDomain #P256 ((fromDomain #P256 (as_nat P256 h0 a) - fromDomain #P256 (as_nat P256 h0 b)) % getPrime P256)))
+
+let felem_sub_p256 a b out = felem_sub_ #P256 a b out
+
+
+val felem_sub_p384: a: felem P384 -> b: felem P384 -> out: felem P384 ->
+  Stack unit
+  (requires (fun h0 ->
+    live h0 out /\ live h0 a /\ live h0 b /\ eq_or_disjoint a out /\ eq_or_disjoint b out /\ eq_or_disjoint a b /\
+    as_nat P384 h0 a < getPrime P384 /\ as_nat P384 h0 b < getPrime P384))
+  (ensures (fun h0 _ h1 -> modifies (loc out) h0 h1 /\
+    as_nat P384 h1 out == (as_nat P384 h0 a - as_nat P384 h0 b) % getPrime P384 /\
+    as_nat P384 h1 out == toDomain #P384 ((fromDomain #P384 (as_nat P384 h0 a) - fromDomain #P384 (as_nat P384 h0 b)) % getPrime P384)))
+
+let felem_sub_p384 a b out = felem_sub_ #P384 a b out
+
+
+val felem_sub_generic: a: felem Default -> b: felem Default -> out: felem Default ->
+  Stack unit
+  (requires (fun h0 ->
+    live h0 out /\ live h0 a /\ live h0 b /\ eq_or_disjoint a out /\ eq_or_disjoint b out /\ eq_or_disjoint a b /\
+    as_nat Default h0 a < getPrime Default /\ as_nat Default h0 b < getPrime Default))
+  (ensures (fun h0 _ h1 -> modifies (loc out) h0 h1 /\
+    as_nat Default h1 out == (as_nat Default h0 a - as_nat Default h0 b) % getPrime Default /\
+    as_nat Default h1 out == toDomain #Default ((fromDomain #Default (as_nat Default h0 a) - fromDomain #Default (as_nat Default h0 b)) % getPrime Default)))
+
+let felem_sub_generic a b out = felem_sub_ #Default a b out
+
+
+let felem_sub #c a b out = 
+  match c with 
+  |P256 -> felem_sub_p256 a b out
+  |P384 -> felem_sub_p384 a b out
+  |Default -> felem_sub_generic a b out
+
 
 
 let mul #c f r out =
